@prefix activity: <http://purl.org/net/ontologies/leisure-activity#>. #needs to be created.  suggested namespace may need to change.
@prefix concept: <http://plings.net/keywords/> . # needs to be created
@base <http://plings.net/a/295421/> . 

@prefix rev: <http://purl.org/stuff/rev#>.
@prefix foaf: <http://xmlns.com/foaf/0.1/>.
@prefix rdf: <http://www.w3.org/1999/02/22-rdf-syntax-ns#>.
@prefix v: <http://www.w3.org/2006/vcard/ns#>.
@prefix dc: <http://purl.org/dc/terms/>.
@prefix skos: <http://www.w3.org/2004/02/skos/core#>.
@prefix geo: <http://www.w3.org/2003/01/geo/wgs84_pos#>.
@prefix rdfs: <http://www.w3.org/2000/01/rdf-schema#> .
@prefix xsd: <http://www.w3.org/2001/XMLSchema#"> .
@prefix owl: <http://www.w3.org/2002/07/owl#>.
@prefix admingeo: <http://data.ordnancesurvey.co.uk/ontology/admingeo/>.
@prefix event: <http://purl.org/NET/c4dm/event.owl#>.
@prefix tl: <http://purl.org/NET/c4dm/timeline.owl#>.
@prefix cal: <http://www.w3.org/2002/12/cal#>.
@prefix gr: <http://purl.org/goodrelations/v1#>.
@prefix postcode: <http://data.ordnancesurvey.co.uk/ontology/postcode/> .


<http://plings.net/a/295421>
	a activity:Activity;
	rdfs:label "Climbing - Teesdale Leisure Centre"@en; 
	gr:hasPriceSpecification <price> ;
#	activity:minAge "10"^^xsd:int; # these age properties are just '0' in the data - I would suggest not outputting  zero/null/Unknown in the RDF, 
                                #  but instead not output the property at all unless there is a meaningful value.
#	activity:maxAge "16"^^xsd:int;
	activity:provider <http://plings.net/o/4863>;
	event:place <http://plings.net/v/59352>;
	event:time <time>; 
	cal:dtstart "2011-01-26T12:00:00"^^xsd:dateTime;
	cal:dtstart "2011-01-26T15:00:00"^^xsd:dateTime;
	activity:contact <http://plings.net/a/295421/contact> ;
  dct:subject  concept:Climbing ;
# activity:relatedActivity <?a> , <?b> ; # this property is not in the data for this record, 
                                         # but is included as an example for other records that do.
.
<price>
	a gr:PriceSpecifcation ;
	gr:hasCurrency "GBP";
	gr:hasCurrencyValue "0.00"^^xsd:float.
<time>
	a tl:Interval;
	tl:at "2011-01-26T12:00:00"^^xsd:dateTime;
	tl:duration "PT3H"^^xsd:duration.

<contact>
	a foaf:Agent;
	foaf:name "Unknown";
	ov:phoneNumber "01833 696 374/01833 696 375";
	ov:postalAddress "Strathmore Rd, Barnard Castle, County Durham, DL12 8DS";
	foaf:mbox <mailto:someone@example.org> ; #this field doesn't have a value in this particular XML record, but is provided as an example
 .

#Categories

#ECM Areas

#Keywords

concept:Climbing a skos:Concept ;
  rdfs:label "Climbing"@en;
  skos:inScheme concept: ;
  skos:broader concept:PhysicalActivity ;
  skos:narrower concept:Bouldering , concept:IndoorClimbing , concept:OutdoorClimbing 
.

concept: a skos:ConceptScheme ;
  rdfs:label "Plings Concept Scheme"@en ;
#  dct:creator <?> ;
  skos:hasTopConcept concept:Activity ;
.

<http://plings.net/v/59352> a activity:Venue ;
  rdfs:label "Teesdale Leisure Centre" ;
  geo:lat 54.551442 ;
  geo:long -1.916745 ;
  v:street-address "Strathmore Road" ;
  v:postal-code "DL12 8DS" ;
  postcode:postcode <http://data.ordnancesurvey.co.uk/id/postcodeunit/DH128DS> ;
  ov:phoneNumber "01833 696 374" ;
  ov:localAuthority <http://statistics.data.gov.uk/doc/local-authority-district/00EJ> ;
  admingeo:ward <http://statistics.data.gov.uk/id/local-authority-ward/00EJME> 
.

#provider
<http://plings.net/o/4863>
  a activity:ActivityProvider ;
  rdfs:label "Get Out There - Durham County Council"@en ;
  dct:description "Get Out There is the Young person's website for things to do and places to go in County Durham. On the website you will find activities which are from sources such as ourselves, community and voluntary sector and private sector organisations. These can be things such as classes at your local leisure centre, film making workshops or events on at your local youth centre. You will find information on the date and time of the event or activity, the location shown on a user friendly map, the facility to enquire online about the activity and how to contact the organisation for more information. There is also regular blogs updating young people on the latest Get Out There news, prizes up for grabs and any new opportunities available. Young people also get the opportunity to add their views by posting comments, suggesting activities or taking part in positive activities surveys. Checks are carried out to ensure that the activities are from trusted sources and that organisations provide the necessary documents to ensure the safety and enjoyment of young people. Get Out There also feeds into the National website for positive activities   Plings, Places To Go, Things to Do  Places and Things  which is a part of the DCSF funded Information and Signposting Project."@en ;
  foaf:page <http://www.getoutthere.info/> ;
  foaf:homepage <http://www.getoutthere.info/> ;
  activity:contact <http://plings.net/o/4863/contact> ;
  v:street-address "County Hall" ;
  v:postal-code "DH1 5UL" ;
  postcode:postcode <http://data.ordnancesurvey.co.uk/id/postcodeunit/DH15UL> ;
.  
<http://plings.net/o/4863/contact>
  a foaf:Agent ;
  foaf:name "Paul Hebron" ;
  foaf:mbox <mailto:paul.hebron@durham.gov.uk> ;
.
  
# Vocabulary

activity: a owl:Ontology ;
  rdfs:label "Activity Ontology"@en ;
  rdfs:comment "This vocabulary contains a small set of terms that describe activities (primarily leisure activities) and the venues at which those activities take place."@en-gb ;
.

activity:Activity
  a rdfs:Class
	rdfs:subClassOf event:Event, gr:Offering;
	rdfs:label "Activity"@en;
	rdfs:comment "A thing to do for the purposes of leisure, perhaps with a particular time and place. For example, Yoga class, Wednesday 7pm, Ashton Leisure Centre."@en; 
  rdfs:isDefinedBy activity:
.

activity:ActivityProvider 
  a rdfs:Class ;
  rdfs:subClassOf foaf:Agent ;
  rdfs:label "Activity Provider"@en ;
  rdfs:comment "The provider of an Activity - typically an Organisation such as a Youth Club, a School, a Sport Centre, etc."@en ;
  rdfs:isDefinedBy activity: ;
.

activity:minAge 
  a owl:DatatypeProperty ;
  rdfs:label "Minimum Age"@en;
  rdfs:isDefinedBy activity: ;
  rdfs:domain activity:Activity ;
  rdfs:comment "The minimum age that a person can be to participate in the activity."@en ;
.

activity:maxAge 
  a owl:DatatypeProperty ;
  rdfs:label "Maximum Age"@en;
  rdfs:isDefinedBy activity: ;
  rdfs:domain activity:Activity ;
  rdfs:comment "The maximum age that a person can be to participate in the activity."@en ;
.

activity:provider 
  a owl:ObjectProperty ;
  rdfs:label "Provider"@en;
  rdfs:isDefinedBy activity: ;
  rdfs:domain activity:Activity ;
  rdfs:range activity:ActivityProvider ;
  rdfs:comment "The provider of an activity"@en ;
.

activity:contact 
  a owl:ObjectProperty ;
  rdfs:label "Contact"@en;
  rdfs:isDefinedBy activity: ;
  rdfs:range foaf:Agent ;
  rdfs:comment "A person or organisation that may be contacted for further details."@en ;
.


activity:relatedActivity 
  a owl:ObjectProperty ;
  rdfs:label "Related Activity"@en;
  rdfs:isDefinedBy activity: ;
  rdfs:range activity:Activity ;
  rdfs:domain activity:Activity ;
  rdfs:comment "An activity that may be of interest to people interested in this activity."@en ;
.


# Activity properties
# activity:minAge
# activity:maxAge
# activity:provider
# activity:contact
# activity:relatedActivity

# openvocab properties (need to be created)
# localAuthority
# phoneNumber
# postalAddress

